bin tree

data-structures/Binary_tree.v
@@ -8,32 +8,38 @@ Notation "∀ A , B" := (forall A , B) (at level 200).
 Notation "∃ A , B" := (exists A , B) (at level 200).
 
 
-Inductive tree (K V: Type) : Type := 
+Definition key := nat.
+Definition cmp := key -> key -> bool.
+
+
+Inductive tree (V: Type) : Type := 
 | Leaf
-| Node (l: tree K V) (key: K) (val: V) (r: tree K V).
+| Node (l: tree V) (k: key) (val: V) (r: tree V).
 
-Arguments Leaf {K V}.
-Arguments Node {K V}.
-
-Definition cmp {K: Type} := K -> K -> bool.
+Arguments Leaf {V}.
+Arguments Node {V}.
 
 
-Fixpoint lookup {K V : Type} (x : K) (t : tree K V) (less: @cmp K) : 
+
+Fixpoint lookup_lt {V : Type} (lt: @cmp) (x : key) (t : tree V)  : 
         option V :=
   match t with
   | Leaf => None
-  | Node l y v r => if (less x y) then lookup x l less
-                 else if (less y x) then lookup x r less
+  | Node l y v r => if (lt x y) then lookup_lt lt x l
+                 else if (lt y x) then lookup_lt lt x r
                      else Some v
   end.
 
-Fixpoint insert {K V : Type} (x : K) (v : V) (t : tree K V) (less: @cmp K) : tree K V :=
+Fixpoint insert_lt {V : Type} (lt: @cmp)  (x : key) (v : V) (t : tree V) : tree V :=
   match t with
   | Leaf => Node Leaf x v Leaf
-  | Node l y v' r => if (less x y) then Node (insert x v l less) y v' r
-                 else if (less y x) then Node l y v' (insert x v r less)
+  | Node l y v' r => if (lt x y) then Node (insert_lt lt x v l) y v' r
+                 else if (lt y x) then Node l y v' (insert_lt lt x v r)
                       else Node l x v r
   end.
+
+Definition lookup {V : Type}:  key -> tree V -> option V := (lookup_lt Nat.ltb) .
+Definition insert {V : Type}:  key -> V -> tree V -> tree V := (insert_lt Nat.ltb) .
 
 
 Module Tests.
@@ -44,16 +50,15 @@ Definition test_tree := Node (Node Leaf 2 "two" (Node Leaf 3 "three" Leaf)) 4 "f
 Example tree_test1 :
      insert 3 "three"
      (insert 2 "two" 
-     (insert 4 "four" Leaf Nat.ltb) 
-     Nat.ltb) Nat.ltb = test_tree.
+     (insert 4 "four" Leaf)) = test_tree.
   Proof. simpl. reflexivity. Qed.
 
 Example tree_test2 :
-     lookup 3 test_tree Nat.ltb = Some "three".
+     lookup 3 test_tree = Some "three".
   Proof. simpl. reflexivity. Qed.
 
 Example tree_test3 :
-lookup 5 test_tree Nat.ltb = None.
+lookup 5 test_tree = None.
 Proof. simpl. reflexivity. Qed.
 End Tests.
 
